# Warrior Level - Addition/Subtraction/Multiplication Problems

## Pattern 1: a × b + c - x = d (Problems 1-17)

1. `2 × 3 + 5 - x = 9`
   - 2 × 3 + 5 - x = 9
   - 6 + 5 - x = 9
   - 11 - x = 9
   - x = 11 - 9
   - x = 2

2. `4 × 2 + 7 - x = 12`
   - 4 × 2 + 7 - x = 12
   - 8 + 7 - x = 12
   - 15 - x = 12
   - x = 15 - 12
   - x = 3

3. `3 × 5 + 4 - x = 15`
   - 3 × 5 + 4 - x = 15
   - 15 + 4 - x = 15
   - 19 - x = 15
   - x = 19 - 15
   - x = 4

4. `6 × 2 + 8 - x = 18`
   - 6 × 2 + 8 - x = 18
   - 12 + 8 - x = 18
   - 20 - x = 18
   - x = 20 - 18
   - x = 2

5. `5 × 3 + 6 - x = 20`
   - 5 × 3 + 6 - x = 20
   - 15 + 6 - x = 20
   - 21 - x = 20
   - x = 21 - 20
   - x = 1

6. `4 × 4 + 5 - x = 19`
   - 4 × 4 + 5 - x = 19
   - 16 + 5 - x = 19
   - 21 - x = 19
   - x = 21 - 19
   - x = 2

7. `7 × 2 + 9 - x = 20`
   - 7 × 2 + 9 - x = 20
   - 14 + 9 - x = 20
   - 23 - x = 20
   - x = 23 - 20
   - x = 3

8. `3 × 6 + 7 - x = 22`
   - 3 × 6 + 7 - x = 22
   - 18 + 7 - x = 22
   - 25 - x = 22
   - x = 25 - 22
   - x = 3

9. `8 × 2 + 4 - x = 18`
   - 8 × 2 + 4 - x = 18
   - 16 + 4 - x = 18
   - 20 - x = 18
   - x = 20 - 18
   - x = 2

10. `5 × 4 + 8 - x = 25`
    - 5 × 4 + 8 - x = 25
    - 20 + 8 - x = 25
    - 28 - x = 25
    - x = 28 - 25
    - x = 3

11. `6 × 3 + 5 - x = 20`
    - 6 × 3 + 5 - x = 20
    - 18 + 5 - x = 20
    - 23 - x = 20
    - x = 23 - 20
    - x = 3

12. `4 × 5 + 6 - x = 24`
    - 4 × 5 + 6 - x = 24
    - 20 + 6 - x = 24
    - 26 - x = 24
    - x = 26 - 24
    - x = 2

13. `7 × 3 + 8 - x = 27`
    - 7 × 3 + 8 - x = 27
    - 21 + 8 - x = 27
    - 29 - x = 27
    - x = 29 - 27
    - x = 2

14. `6 × 4 + 7 - x = 28`
    - 6 × 4 + 7 - x = 28
    - 24 + 7 - x = 28
    - 31 - x = 28
    - x = 31 - 28
    - x = 3

15. `8 × 3 + 5 - x = 26`
    - 8 × 3 + 5 - x = 26
    - 24 + 5 - x = 26
    - 29 - x = 26
    - x = 29 - 26
    - x = 3

16. `5 × 5 + 9 - x = 32`
    - 5 × 5 + 9 - x = 32
    - 25 + 9 - x = 32
    - 34 - x = 32
    - x = 34 - 32
    - x = 2

17. `9 × 2 + 6 - x = 22`
    - 9 × 2 + 6 - x = 22
    - 18 + 6 - x = 22
    - 24 - x = 22
    - x = 24 - 22
    - x = 2

## Pattern 2: a × b - c + x = d (Problems 18-34)

18. `3 × 4 - 5 + x = 12`
    - 3 × 4 - 5 + x = 12
    - 12 - 5 + x = 12
    - 7 + x = 12
    - x = 12 - 7
    - x = 5

19. `5 × 3 - 8 + x = 15`
    - 5 × 3 - 8 + x = 15
    - 15 - 8 + x = 15
    - 7 + x = 15
    - x = 15 - 7
    - x = 8

20. `4 × 4 - 6 + x = 18`
    - 4 × 4 - 6 + x = 18
    - 16 - 6 + x = 18
    - 10 + x = 18
    - x = 18 - 10
    - x = 8

21. `6 × 2 - 4 + x = 14`
    - 6 × 2 - 4 + x = 14
    - 12 - 4 + x = 14
    - 8 + x = 14
    - x = 14 - 8
    - x = 6

22. `7 × 3 - 9 + x = 20`
    - 7 × 3 - 9 + x = 20
    - 21 - 9 + x = 20
    - 12 + x = 20
    - x = 20 - 12
    - x = 8

23. `5 × 4 - 7 + x = 22`
    - 5 × 4 - 7 + x = 22
    - 20 - 7 + x = 22
    - 13 + x = 22
    - x = 22 - 13
    - x = 9

24. `8 × 2 - 5 + x = 19`
    - 8 × 2 - 5 + x = 19
    - 16 - 5 + x = 19
    - 11 + x = 19
    - x = 19 - 11
    - x = 8

25. `6 × 3 - 8 + x = 20`
    - 6 × 3 - 8 + x = 20
    - 18 - 8 + x = 20
    - 10 + x = 20
    - x = 20 - 10
    - x = 10

26. `4 × 5 - 6 + x = 24`
    - 4 × 5 - 6 + x = 24
    - 20 - 6 + x = 24
    - 14 + x = 24
    - x = 24 - 14
    - x = 10

27. `9 × 2 - 7 + x = 21`
    - 9 × 2 - 7 + x = 21
    - 18 - 7 + x = 21
    - 11 + x = 21
    - x = 21 - 11
    - x = 10

28. `7 × 4 - 10 + x = 28`
    - 7 × 4 - 10 + x = 28
    - 28 - 10 + x = 28
    - 18 + x = 28
    - x = 28 - 18
    - x = 10

29. `8 × 3 - 9 + x = 25`
    - 8 × 3 - 9 + x = 25
    - 24 - 9 + x = 25
    - 15 + x = 25
    - x = 25 - 15
    - x = 10

30. `6 × 4 - 8 + x = 26`
    - 6 × 4 - 8 + x = 26
    - 24 - 8 + x = 26
    - 16 + x = 26
    - x = 26 - 16
    - x = 10

31. `5 × 6 - 12 + x = 30`
    - 5 × 6 - 12 + x = 30
    - 30 - 12 + x = 30
    - 18 + x = 30
    - x = 30 - 18
    - x = 12

32. `9 × 3 - 11 + x = 28`
    - 9 × 3 - 11 + x = 28
    - 27 - 11 + x = 28
    - 16 + x = 28
    - x = 28 - 16
    - x = 12

33. `7 × 5 - 15 + x = 35`
    - 7 × 5 - 15 + x = 35
    - 35 - 15 + x = 35
    - 20 + x = 35
    - x = 35 - 20
    - x = 15

34. `8 × 4 - 12 + x = 32`
    - 8 × 4 - 12 + x = 32
    - 32 - 12 + x = 32
    - 20 + x = 32
    - x = 32 - 20
    - x = 12

## Pattern 3: a + b × c - x = d (Problems 35-50)

35. `5 + 3 × 4 - x = 14`
    - 5 + 3 × 4 - x = 14
    - 5 + 12 - x = 14
    - 17 - x = 14
    - x = 17 - 14
    - x = 3

36. `8 + 2 × 6 - x = 18`
    - 8 + 2 × 6 - x = 18
    - 8 + 12 - x = 18
    - 20 - x = 18
    - x = 20 - 18
    - x = 2

37. `6 + 4 × 3 - x = 16`
    - 6 + 4 × 3 - x = 16
    - 6 + 12 - x = 16
    - 18 - x = 16
    - x = 18 - 16
    - x = 2

38. `10 + 3 × 5 - x = 22`
    - 10 + 3 × 5 - x = 22
    - 10 + 15 - x = 22
    - 25 - x = 22
    - x = 25 - 22
    - x = 3

39. `7 + 5 × 2 - x = 15`
    - 7 + 5 × 2 - x = 15
    - 7 + 10 - x = 15
    - 17 - x = 15
    - x = 17 - 15
    - x = 2

40. `12 + 4 × 3 - x = 22`
    - 12 + 4 × 3 - x = 22
    - 12 + 12 - x = 22
    - 24 - x = 22
    - x = 24 - 22
    - x = 2

41. `9 + 6 × 2 - x = 19`
    - 9 + 6 × 2 - x = 19
    - 9 + 12 - x = 19
    - 21 - x = 19
    - x = 21 - 19
    - x = 2

42. `15 + 3 × 4 - x = 25`
    - 15 + 3 × 4 - x = 25
    - 15 + 12 - x = 25
    - 27 - x = 25
    - x = 27 - 25
    - x = 2

43. `11 + 5 × 3 - x = 24`
    - 11 + 5 × 3 - x = 24
    - 11 + 15 - x = 24
    - 26 - x = 24
    - x = 26 - 24
    - x = 2

44. `8 + 7 × 2 - x = 20`
    - 8 + 7 × 2 - x = 20
    - 8 + 14 - x = 20
    - 22 - x = 20
    - x = 22 - 20
    - x = 2

45. `14 + 4 × 4 - x = 28`
    - 14 + 4 × 4 - x = 28
    - 14 + 16 - x = 28
    - 30 - x = 28
    - x = 30 - 28
    - x = 2

46. `13 + 6 × 3 - x = 29`
    - 13 + 6 × 3 - x = 29
    - 13 + 18 - x = 29
    - 31 - x = 29
    - x = 31 - 29
    - x = 2

47. `16 + 5 × 4 - x = 34`
    - 16 + 5 × 4 - x = 34
    - 16 + 20 - x = 34
    - 36 - x = 34
    - x = 36 - 34
    - x = 2

48. `18 + 3 × 6 - x = 34`
    - 18 + 3 × 6 - x = 34
    - 18 + 18 - x = 34
    - 36 - x = 34
    - x = 36 - 34
    - x = 2

49. `20 + 4 × 5 - x = 38`
    - 20 + 4 × 5 - x = 38
    - 20 + 20 - x = 38
    - 40 - x = 38
    - x = 40 - 38
    - x = 2

50. `17 + 7 × 3 - x = 36`
    - 17 + 7 × 3 - x = 36
    - 17 + 21 - x = 36
    - 38 - x = 36
    - x = 38 - 36
    - x = 2
