# Beginner Level - Addition/Subtraction Problems

## Pattern 1: a + b - x = c (Problems 1-17)

1. `5 + 3 - x = 6`
   - 5 + 3 - x = 6
   - 8 - x = 6
   - x = 8 - 6
   - x = 2

2. `8 + 4 - x = 9`
   - 8 + 4 - x = 9
   - 12 - x = 9
   - x = 12 - 9
   - x = 3

3. `7 + 6 - x = 8`
   - 7 + 6 - x = 8
   - 13 - x = 8
   - x = 13 - 8
   - x = 5

4. `9 + 5 - x = 11`
   - 9 + 5 - x = 11
   - 14 - x = 11
   - x = 14 - 11
   - x = 3

5. `12 + 8 - x = 15`
   - 12 + 8 - x = 15
   - 20 - x = 15
   - x = 20 - 15
   - x = 5

6. `10 + 7 - x = 12`
   - 10 + 7 - x = 12
   - 17 - x = 12
   - x = 17 - 12
   - x = 5

7. `15 + 9 - x = 18`
   - 15 + 9 - x = 18
   - 24 - x = 18
   - x = 24 - 18
   - x = 6

8. `14 + 11 - x = 20`
   - 14 + 11 - x = 20
   - 25 - x = 20
   - x = 25 - 20
   - x = 5

9. `18 + 12 - x = 25`
   - 18 + 12 - x = 25
   - 30 - x = 25
   - x = 30 - 25
   - x = 5

10. `20 + 15 - x = 28`
    - 20 + 15 - x = 28
    - 35 - x = 28
    - x = 35 - 28
    - x = 7

11. `16 + 13 - x = 22`
    - 16 + 13 - x = 22
    - 29 - x = 22
    - x = 29 - 22
    - x = 7

12. `22 + 18 - x = 32`
    - 22 + 18 - x = 32
    - 40 - x = 32
    - x = 40 - 32
    - x = 8

13. `25 + 20 - x = 38`
    - 25 + 20 - x = 38
    - 45 - x = 38
    - x = 45 - 38
    - x = 7

14. `30 + 25 - x = 45`
    - 30 + 25 - x = 45
    - 55 - x = 45
    - x = 55 - 45
    - x = 10

15. `28 + 22 - x = 42`
    - 28 + 22 - x = 42
    - 50 - x = 42
    - x = 50 - 42
    - x = 8

16. `35 + 28 - x = 55`
    - 35 + 28 - x = 55
    - 63 - x = 55
    - x = 63 - 55
    - x = 8

17. `40 + 32 - x = 65`
    - 40 + 32 - x = 65
    - 72 - x = 65
    - x = 72 - 65
    - x = 7

## Pattern 2: a - b + x = c (Problems 18-34)

18. `10 - 3 + x = 12`
    - 10 - 3 + x = 12
    - 7 + x = 12
    - x = 12 - 7
    - x = 5

19. `15 - 5 + x = 18`
    - 15 - 5 + x = 18
    - 10 + x = 18
    - x = 18 - 10
    - x = 8

20. `20 - 8 + x = 25`
    - 20 - 8 + x = 25
    - 12 + x = 25
    - x = 25 - 12
    - x = 13

21. `18 - 6 + x = 22`
    - 18 - 6 + x = 22
    - 12 + x = 22
    - x = 22 - 12
    - x = 10

22. `25 - 9 + x = 30`
    - 25 - 9 + x = 30
    - 16 + x = 30
    - x = 30 - 16
    - x = 14

23. `30 - 12 + x = 35`
    - 30 - 12 + x = 35
    - 18 + x = 35
    - x = 35 - 18
    - x = 17

24. `28 - 10 + x = 38`
    - 28 - 10 + x = 38
    - 18 + x = 38
    - x = 38 - 18
    - x = 20

25. `35 - 15 + x = 45`
    - 35 - 15 + x = 45
    - 20 + x = 45
    - x = 45 - 20
    - x = 25

26. `40 - 18 + x = 50`
    - 40 - 18 + x = 50
    - 22 + x = 50
    - x = 50 - 22
    - x = 28

27. `45 - 20 + x = 55`
    - 45 - 20 + x = 55
    - 25 + x = 55
    - x = 55 - 25
    - x = 30

28. `50 - 22 + x = 65`
    - 50 - 22 + x = 65
    - 28 + x = 65
    - x = 65 - 28
    - x = 37

29. `55 - 25 + x = 70`
    - 55 - 25 + x = 70
    - 30 + x = 70
    - x = 70 - 30
    - x = 40

30. `60 - 28 + x = 75`
    - 60 - 28 + x = 75
    - 32 + x = 75
    - x = 75 - 32
    - x = 43

31. `65 - 30 + x = 80`
    - 65 - 30 + x = 80
    - 35 + x = 80
    - x = 80 - 35
    - x = 45

32. `70 - 35 + x = 85`
    - 70 - 35 + x = 85
    - 35 + x = 85
    - x = 85 - 35
    - x = 50

33. `75 - 40 + x = 90`
    - 75 - 40 + x = 90
    - 35 + x = 90
    - x = 90 - 35
    - x = 55

34. `80 - 45 + x = 95`
    - 80 - 45 + x = 95
    - 35 + x = 95
    - x = 95 - 35
    - x = 60

## Pattern 3: a + b - c = x (Problems 35-50)

35. `8 + 5 - 3 = x`
    - 8 + 5 - 3 = x
    - 13 - 3 = x
    - x = 10

36. `12 + 7 - 5 = x`
    - 12 + 7 - 5 = x
    - 19 - 5 = x
    - x = 14

37. `15 + 9 - 8 = x`
    - 15 + 9 - 8 = x
    - 24 - 8 = x
    - x = 16

38. `18 + 12 - 10 = x`
    - 18 + 12 - 10 = x
    - 30 - 10 = x
    - x = 20

39. `20 + 15 - 12 = x`
    - 20 + 15 - 12 = x
    - 35 - 12 = x
    - x = 23

40. `25 + 18 - 15 = x`
    - 25 + 18 - 15 = x
    - 43 - 15 = x
    - x = 28

41. `30 + 22 - 18 = x`
    - 30 + 22 - 18 = x
    - 52 - 18 = x
    - x = 34

42. `35 + 25 - 20 = x`
    - 35 + 25 - 20 = x
    - 60 - 20 = x
    - x = 40

43. `40 + 28 - 25 = x`
    - 40 + 28 - 25 = x
    - 68 - 25 = x
    - x = 43

44. `45 + 32 - 28 = x`
    - 45 + 32 - 28 = x
    - 77 - 28 = x
    - x = 49

45. `50 + 35 - 30 = x`
    - 50 + 35 - 30 = x
    - 85 - 30 = x
    - x = 55

46. `55 + 40 - 35 = x`
    - 55 + 40 - 35 = x
    - 95 - 35 = x
    - x = 60

47. `60 + 45 - 40 = x`
    - 60 + 45 - 40 = x
    - 105 - 40 = x
    - x = 65

48. `65 + 50 - 45 = x`
    - 65 + 50 - 45 = x
    - 115 - 45 = x
    - x = 70

49. `70 + 55 - 50 = x`
    - 70 + 55 - 50 = x
    - 125 - 50 = x
    - x = 75

50. `75 + 60 - 55 = x`
    - 75 + 60 - 55 = x
    - 135 - 55 = x
    - x = 80
