# Master Level - Addition/Subtraction/Multiplication/Division Problems

## Pattern 1: a × b ÷ c + d - X = e (Problems 1-13)

1. `6 × 4 ÷ 2 + 5 - X = 16`
   - 6 × 4 ÷ 2 + 5 - X = 16
   - 24 ÷ 2 + 5 - X = 16
   - 12 + 5 - X = 16
   - 17 - X = 16
   - X = 17 - 16
   - X = 1

2. `8 × 3 ÷ 4 + 7 - X = 13`
   - 8 × 3 ÷ 4 + 7 - X = 13
   - 24 ÷ 4 + 7 - X = 13
   - 6 + 7 - X = 13
   - 13 - X = 13
   - X = 13 - 13
   - X = 0

3. `12 × 2 ÷ 3 + 4 - X = 12`
   - 12 × 2 ÷ 3 + 4 - X = 12
   - 24 ÷ 3 + 4 - X = 12
   - 8 + 4 - X = 12
   - 12 - X = 12
   - X = 12 - 12
   - X = 0

4. `15 × 2 ÷ 5 + 8 - X = 14`
   - 15 × 2 ÷ 5 + 8 - X = 14
   - 30 ÷ 5 + 8 - X = 14
   - 6 + 8 - X = 14
   - 14 - X = 14
   - X = 14 - 14
   - X = 0

5. `18 × 2 ÷ 6 + 9 - X = 15`
   - 18 × 2 ÷ 6 + 9 - X = 15
   - 36 ÷ 6 + 9 - X = 15
   - 6 + 9 - X = 15
   - 15 - X = 15
   - X = 15 - 15
   - X = 0

6. `20 × 3 ÷ 4 + 6 - X = 21`
   - 20 × 3 ÷ 4 + 6 - X = 21
   - 60 ÷ 4 + 6 - X = 21
   - 15 + 6 - X = 21
   - 21 - X = 21
   - X = 21 - 21
   - X = 0

7. `14 × 3 ÷ 7 + 5 - X = 11`
   - 14 × 3 ÷ 7 + 5 - X = 11
   - 42 ÷ 7 + 5 - X = 11
   - 6 + 5 - X = 11
   - 11 - X = 11
   - X = 11 - 11
   - X = 0

8. `16 × 2 ÷ 8 + 7 - X = 11`
   - 16 × 2 ÷ 8 + 7 - X = 11
   - 32 ÷ 8 + 7 - X = 11
   - 4 + 7 - X = 11
   - 11 - X = 11
   - X = 11 - 11
   - X = 0

9. `21 × 2 ÷ 3 + 4 - X = 18`
   - 21 × 2 ÷ 3 + 4 - X = 18
   - 42 ÷ 3 + 4 - X = 18
   - 14 + 4 - X = 18
   - 18 - X = 18
   - X = 18 - 18
   - X = 0

10. `24 × 2 ÷ 6 + 8 - X = 16`
    - 24 × 2 ÷ 6 + 8 - X = 16
    - 48 ÷ 6 + 8 - X = 16
    - 8 + 8 - X = 16
    - 16 - X = 16
    - X = 16 - 16
    - X = 0

11. `27 × 2 ÷ 9 + 5 - X = 11`
    - 27 × 2 ÷ 9 + 5 - X = 11
    - 54 ÷ 9 + 5 - X = 11
    - 6 + 5 - X = 11
    - 11 - X = 11
    - X = 11 - 11
    - X = 0

12. `30 × 2 ÷ 5 + 7 - X = 19`
    - 30 × 2 ÷ 5 + 7 - X = 19
    - 60 ÷ 5 + 7 - X = 19
    - 12 + 7 - X = 19
    - 19 - X = 19
    - X = 19 - 19
    - X = 0

13. `28 × 3 ÷ 7 + 9 - X = 21`
    - 28 × 3 ÷ 7 + 9 - X = 21
    - 84 ÷ 7 + 9 - X = 21
    - 12 + 9 - X = 21
    - 21 - X = 21
    - X = 21 - 21
    - X = 0

## Pattern 2: a × b ÷ c - d + X = e (Problems 14-25)

14. `12 × 4 ÷ 6 - 3 + X = 12`
    - 12 × 4 ÷ 6 - 3 + X = 12
    - 48 ÷ 6 - 3 + X = 12
    - 8 - 3 + X = 12
    - 5 + X = 12
    - X = 12 - 5
    - X = 7

15. `18 × 2 ÷ 3 - 5 + X = 13`
    - 18 × 2 ÷ 3 - 5 + X = 13
    - 36 ÷ 3 - 5 + X = 13
    - 12 - 5 + X = 13
    - 7 + X = 13
    - X = 13 - 7
    - X = 6

16. `24 × 3 ÷ 8 - 4 + X = 11`
    - 24 × 3 ÷ 8 - 4 + X = 11
    - 72 ÷ 8 - 4 + X = 11
    - 9 - 4 + X = 11
    - 5 + X = 11
    - X = 11 - 5
    - X = 6

17. `20 × 2 ÷ 5 - 6 + X = 10`
    - 20 × 2 ÷ 5 - 6 + X = 10
    - 40 ÷ 5 - 6 + X = 10
    - 8 - 6 + X = 10
    - 2 + X = 10
    - X = 10 - 2
    - X = 8

18. `15 × 4 ÷ 5 - 7 + X = 11`
    - 15 × 4 ÷ 5 - 7 + X = 11
    - 60 ÷ 5 - 7 + X = 11
    - 12 - 7 + X = 11
    - 5 + X = 11
    - X = 11 - 5
    - X = 6

19. `32 × 2 ÷ 8 - 3 + X = 9`
    - 32 × 2 ÷ 8 - 3 + X = 9
    - 64 ÷ 8 - 3 + X = 9
    - 8 - 3 + X = 9
    - 5 + X = 9
    - X = 9 - 5
    - X = 4

20. `21 × 3 ÷ 7 - 5 + X = 13`
    - 21 × 3 ÷ 7 - 5 + X = 13
    - 63 ÷ 7 - 5 + X = 13
    - 9 - 5 + X = 13
    - 4 + X = 13
    - X = 13 - 4
    - X = 9

21. `36 × 2 ÷ 9 - 4 + X = 12`
    - 36 × 2 ÷ 9 - 4 + X = 12
    - 72 ÷ 9 - 4 + X = 12
    - 8 - 4 + X = 12
    - 4 + X = 12
    - X = 12 - 4
    - X = 8

22. `25 × 2 ÷ 5 - 8 + X = 14`
    - 25 × 2 ÷ 5 - 8 + X = 14
    - 50 ÷ 5 - 8 + X = 14
    - 10 - 8 + X = 14
    - 2 + X = 14
    - X = 14 - 2
    - X = 12

23. `42 × 2 ÷ 7 - 6 + X = 16`
    - 42 × 2 ÷ 7 - 6 + X = 16
    - 84 ÷ 7 - 6 + X = 16
    - 12 - 6 + X = 16
    - 6 + X = 16
    - X = 16 - 6
    - X = 10

24. `48 × 2 ÷ 8 - 9 + X = 15`
    - 48 × 2 ÷ 8 - 9 + X = 15
    - 96 ÷ 8 - 9 + X = 15
    - 12 - 9 + X = 15
    - 3 + X = 15
    - X = 15 - 3
    - X = 12

25. `35 × 2 ÷ 7 - 4 + X = 16`
    - 35 × 2 ÷ 7 - 4 + X = 16
    - 70 ÷ 7 - 4 + X = 16
    - 10 - 4 + X = 16
    - 6 + X = 16
    - X = 16 - 6
    - X = 10

## Pattern 3: a + b × c ÷ d - X = e (Problems 26-38)

26. `8 + 12 × 2 ÷ 3 - X = 16`
    - 8 + 12 × 2 ÷ 3 - X = 16
    - 8 + 24 ÷ 3 - X = 16
    - 8 + 8 - X = 16
    - 16 - X = 16
    - X = 16 - 16
    - X = 0

27. `10 + 15 × 4 ÷ 5 - X = 22`
    - 10 + 15 × 4 ÷ 5 - X = 22
    - 10 + 60 ÷ 5 - X = 22
    - 10 + 12 - X = 22
    - 22 - X = 22
    - X = 22 - 22
    - X = 0

28. `12 + 18 × 2 ÷ 6 - X = 18`
    - 12 + 18 × 2 ÷ 6 - X = 18
    - 12 + 36 ÷ 6 - X = 18
    - 12 + 6 - X = 18
    - 18 - X = 18
    - X = 18 - 18
    - X = 0

29. `15 + 20 × 3 ÷ 4 - X = 30`
    - 15 + 20 × 3 ÷ 4 - X = 30
    - 15 + 60 ÷ 4 - X = 30
    - 15 + 15 - X = 30
    - 30 - X = 30
    - X = 30 - 30
    - X = 0

30. `6 + 21 × 2 ÷ 7 - X = 12`
    - 6 + 21 × 2 ÷ 7 - X = 12
    - 6 + 42 ÷ 7 - X = 12
    - 6 + 6 - X = 12
    - 12 - X = 12
    - X = 12 - 12
    - X = 0

31. `18 + 24 × 3 ÷ 8 - X = 27`
    - 18 + 24 × 3 ÷ 8 - X = 27
    - 18 + 72 ÷ 8 - X = 27
    - 18 + 9 - X = 27
    - 27 - X = 27
    - X = 27 - 27
    - X = 0

32. `14 + 25 × 2 ÷ 5 - X = 24`
    - 14 + 25 × 2 ÷ 5 - X = 24
    - 14 + 50 ÷ 5 - X = 24
    - 14 + 10 - X = 24
    - 24 - X = 24
    - X = 24 - 24
    - X = 0

33. `20 + 28 × 3 ÷ 7 - X = 32`
    - 20 + 28 × 3 ÷ 7 - X = 32
    - 20 + 84 ÷ 7 - X = 32
    - 20 + 12 - X = 32
    - 32 - X = 32
    - X = 32 - 32
    - X = 0

34. `16 + 30 × 2 ÷ 6 - X = 26`
    - 16 + 30 × 2 ÷ 6 - X = 26
    - 16 + 60 ÷ 6 - X = 26
    - 16 + 10 - X = 26
    - 26 - X = 26
    - X = 26 - 26
    - X = 0

35. `22 + 32 × 3 ÷ 8 - X = 34`
    - 22 + 32 × 3 ÷ 8 - X = 34
    - 22 + 96 ÷ 8 - X = 34
    - 22 + 12 - X = 34
    - 34 - X = 34
    - X = 34 - 34
    - X = 0

36. `25 + 35 × 2 ÷ 7 - X = 35`
    - 25 + 35 × 2 ÷ 7 - X = 35
    - 25 + 70 ÷ 7 - X = 35
    - 25 + 10 - X = 35
    - 35 - X = 35
    - X = 35 - 35
    - X = 0

37. `30 + 36 × 4 ÷ 9 - X = 46`
    - 30 + 36 × 4 ÷ 9 - X = 46
    - 30 + 144 ÷ 9 - X = 46
    - 30 + 16 - X = 46
    - 46 - X = 46
    - X = 46 - 46
    - X = 0

38. `28 + 40 × 3 ÷ 8 - X = 43`
    - 28 + 40 × 3 ÷ 8 - X = 43
    - 28 + 120 ÷ 8 - X = 43
    - 28 + 15 - X = 43
    - 43 - X = 43
    - X = 43 - 43
    - X = 0

## Pattern 4: a - b × c ÷ d + X = e (Problems 39-50)

39. `20 - 12 × 2 ÷ 3 + X = 16`
    - 20 - 12 × 2 ÷ 3 + X = 16
    - 20 - 24 ÷ 3 + X = 16
    - 20 - 8 + X = 16
    - 12 + X = 16
    - X = 16 - 12
    - X = 4

40. `25 - 15 × 4 ÷ 5 + X = 19`
    - 25 - 15 × 4 ÷ 5 + X = 19
    - 25 - 60 ÷ 5 + X = 19
    - 25 - 12 + X = 19
    - 13 + X = 19
    - X = 19 - 13
    - X = 6

41. `30 - 18 × 2 ÷ 6 + X = 27`
    - 30 - 18 × 2 ÷ 6 + X = 27
    - 30 - 36 ÷ 6 + X = 27
    - 30 - 6 + X = 27
    - 24 + X = 27
    - X = 27 - 24
    - X = 3

42. `28 - 20 × 3 ÷ 4 + X = 24`
    - 28 - 20 × 3 ÷ 4 + X = 24
    - 28 - 60 ÷ 4 + X = 24
    - 28 - 15 + X = 24
    - 13 + X = 24
    - X = 24 - 13
    - X = 11

43. `35 - 21 × 2 ÷ 7 + X = 32`
    - 35 - 21 × 2 ÷ 7 + X = 32
    - 35 - 42 ÷ 7 + X = 32
    - 35 - 6 + X = 32
    - 29 + X = 32
    - X = 32 - 29
    - X = 3

44. `40 - 24 × 3 ÷ 8 + X = 37`
    - 40 - 24 × 3 ÷ 8 + X = 37
    - 40 - 72 ÷ 8 + X = 37
    - 40 - 9 + X = 37
    - 31 + X = 37
    - X = 37 - 31
    - X = 6

45. `32 - 25 × 2 ÷ 5 + X = 26`
    - 32 - 25 × 2 ÷ 5 + X = 26
    - 32 - 50 ÷ 5 + X = 26
    - 32 - 10 + X = 26
    - 22 + X = 26
    - X = 26 - 22
    - X = 4

46. `45 - 28 × 3 ÷ 7 + X = 39`
    - 45 - 28 × 3 ÷ 7 + X = 39
    - 45 - 84 ÷ 7 + X = 39
    - 45 - 12 + X = 39
    - 33 + X = 39
    - X = 39 - 33
    - X = 6

47. `38 - 30 × 2 ÷ 6 + X = 33`
    - 38 - 30 × 2 ÷ 6 + X = 33
    - 38 - 60 ÷ 6 + X = 33
    - 38 - 10 + X = 33
    - 28 + X = 33
    - X = 33 - 28
    - X = 5

48. `50 - 32 × 3 ÷ 8 + X = 44`
    - 50 - 32 × 3 ÷ 8 + X = 44
    - 50 - 96 ÷ 8 + X = 44
    - 50 - 12 + X = 44
    - 38 + X = 44
    - X = 44 - 38
    - X = 6

49. `42 - 35 × 2 ÷ 7 + X = 36`
    - 42 - 35 × 2 ÷ 7 + X = 36
    - 42 - 70 ÷ 7 + X = 36
    - 42 - 10 + X = 36
    - 32 + X = 36
    - X = 36 - 32
    - X = 4

50. `48 - 36 × 4 ÷ 9 + X = 36`
    - 48 - 36 × 4 ÷ 9 + X = 36
    - 48 - 144 ÷ 9 + X = 36
    - 48 - 16 + X = 36
    - 32 + X = 36
    - X = 36 - 32
    - X = 4
